FokkerChallenge.lean
@@ -14,6 +14,7 @@ import FokkerChallenge.EnhancedCslib.BetaEtaNormalForm
 import FokkerChallenge.EnhancedCslib.FvarSubset
 import FokkerChallenge.EnhancedCslib.ReflTransGenWithSteps
 import FokkerChallenge.EnhancedCslib.LeftMost
+import FokkerChallenge.EnhancedCslib.Closedunderapp
 import FokkerChallenge.Decider.NoDuplicate
 import FokkerChallenge.Decider.EveryBvarUsed
 import FokkerChallenge.Decider.All0
