FokkerChallenge/EnhancedCslib/Closedunderapp.lean
@@ -1,0 +1,45 @@
+import Cslib.Languages.LambdaCalculus.LocallyNameless.Untyped.Basic
+import Cslib.Languages.LambdaCalculus.LocallyNameless.Untyped.LcAt
+
+namespace Cslib
+
+namespace LambdaCalculus.LocallyNameless.Untyped.Term
+
+@[scoped grind]
+inductive ClosedUnderApp (P: Term String -> Prop): Term String -> Prop where
+  | base {a}: P a -> ClosedUnderApp P a
+  | app {a b}: ClosedUnderApp P a -> ClosedUnderApp P b -> ClosedUnderApp P (.app a b)
+
+theorem closedunderapp_multiapp {Q} {M : Term String}
+  (h2 : ClosedUnderApp Q M) :
+  ∃ (l: List (Term String)) (f : Term String), M = l.foldl Term.app f /\ Q f /\ ∀ x ∈ l, ClosedUnderApp Q x := by
+  induction h2 with
+  | base _ => rename_i M _
+              exists []
+              exists M
+              grind
+  | app _ _ iha ihb =>
+      rename_i a b _ _
+      obtain ⟨la, fa, iha⟩ := iha
+      obtain ⟨lb, fb, ihb⟩ := ihb
+      exists (la ++ [b])
+      exists fa
+      grind
+
+theorem closedunderapp_multiapp_cons {l : List (Term String)} {Q} {f: Term String}:
+  (∀ x ∈ l, ClosedUnderApp Q x) ->
+  ClosedUnderApp Q f ->
+  ClosedUnderApp Q (l.foldl Term.app f) := by
+  induction l generalizing f with
+  | nil => grind
+  | cons head tail ih =>
+    intros _ _
+    simp
+    apply ih <;> grind
+
+@[scoped grind]
+theorem closedunderapp_lc {Q} {M : Term String}
+  (h : ∀ x, Q x -> x.LC)
+  (h2 : ClosedUnderApp Q M) :
+  M.LC := by
+  induction h2 with grind
